compiler/src/MemoryLayout.v
@@ -1,0 +1,30 @@
+Require Import Coq.ZArith.ZArith.
+Require Import coqutil.Word.Interface.
+
+Open Scope Z_scope.
+
+Section Params1.
+  Context {width: Z} {word: word.word width}.
+
+  Record MemoryLayout: Type := {
+    code_start: word;
+    code_pastend: word;
+    heap_start: word;
+    heap_pastend: word;
+    stack_start: word;
+    stack_pastend: word;
+  }.
+
+  (* Could also just require disjointness but <= is simpler to state *)
+  Record MemoryLayoutOk(ml: MemoryLayout): Prop := {
+    code_start_aligned: (word.unsigned ml.(code_start)) mod 4 = 0;
+    code_pastend_ok: word.unsigned ml.(code_start) <= word.unsigned ml.(code_pastend);
+    heap_after_code: word.unsigned ml.(code_pastend) <= word.unsigned ml.(heap_start);
+    heap_pastend_ok: word.unsigned ml.(heap_start) <= word.unsigned ml.(heap_pastend);
+    stack_after_heap: word.unsigned ml.(heap_pastend) <= word.unsigned ml.(stack_start);
+    stack_pastend_ok: word.unsigned ml.(stack_start) <= word.unsigned ml.(stack_pastend);
+  }.
+
+End Params1.
+
+Arguments MemoryLayout _ {_}.
